add modal logic S4

src/mpl/encoding.lean
@@ -4,7 +4,7 @@ Released under the Apache License 2.0 (see "License");
 Author: Bruno Bentzen
 -/
 
-import ..prime data.encodable .syntax.language.basic
+import data.equiv.encodable .default 
 
 open form nat list decidable 
 
@@ -17,6 +17,7 @@ def encode_form : form σ → nat
 | (atom v)   := 3^(v.1 + 1)
 |  (bot σ)   := 2
 | (impl p q) := 5^(encode_form p) * 7^(encode_form q)
+| (box p)   := 11^(encode_form p)
 
 /- our encoding is well behaved -/
 
@@ -26,13 +27,16 @@ list.rec_on (factors n) true (λ n _ ih, if n = 3 then ih else false)
 def is_impl (n : nat) : Prop :=
 list.rec_on (factors n) true (λ n _ ih, if n = 5 ∨ n = 7 then ih else false)
 
+def is_box (n : nat) : Prop :=
+list.rec_on (factors n) true (λ n _ ih, if n = 11 then ih else false)
+
 instance is_atom_dec {n : nat} : decidable (is_atom n) :=
 begin
   induction n, simp,
     apply is_true, trivial,
     unfold is_atom ite, induction factors (succ n_n),
       simp, apply is_true, trivial,
-      simp, induction (nat.decidable_eq hd 3),
+      simp, induction (nat.decidable_eq hd _),
         simp, apply is_false, apply id,
         simp, assumption
 end
@@ -51,13 +55,24 @@ begin
         }
 end
 
+instance is_box_dec {n : nat} : decidable (is_box n) :=
+begin
+  induction n, simp,
+    apply is_true, trivial,
+    unfold is_box ite, induction factors (succ n_n),
+      simp, apply is_true, trivial,
+      simp, induction (nat.decidable_eq hd _),
+        simp, apply is_false, apply id,
+        simp, assumption
+end
+
 def encode_ge_one : ∀ (p : form σ), encode_form p ≥ 1
-| (#v) := by apply nat.le_trans (succ_le_succ (zero_le 1)); apply prime_exp_le prime_three
+| (#v) := by apply nat.le_trans (succ_le_succ (nat.zero_le 1)); apply prime_exp_le prime_three
 | (bot σ) := dec_trivial
-| (p ⊃ q) := 
-  by apply nat.le_trans (succ_le_succ (zero_le 1)); 
-  apply prime_double_exp_le prime_five prime_seven
-  (encode_ge_one p) (encode_ge_one q)
+| (p ⊃ q) := by apply nat.le_trans (succ_le_succ (nat.zero_le 1)); apply prime_double_exp_le prime_five prime_seven (encode_ge_one p) (encode_ge_one q)
+| (◻p) :=
+  by apply nat.le_trans (succ_le_succ (nat.zero_le 1)); unfold encode_form; cases le.dest (encode_ge_one p);
+    rw nat.add_comm at h; rw h.symm; apply prime_exp_le prime_eleven
 
 def is_atom_pow_three : ∀ (n : ℕ), is_atom (3^n)
 | 0 := by unfold is_atom ite
@@ -67,6 +82,14 @@ def not_atom_pow_five_seven  {n m : ℕ } : ¬ is_atom (5^(n+1) * 7^(m+1)) :=
 have ¬ 5 = 3 := dec_trivial,
 by unfold is_atom ite; rw factors_of_double_exp_prime prime_five prime_seven (le_succ 6);
   simp; induction nat.decidable_eq _ _; simp; contradiction
+
+def not_atom_pow_eleven (n > 0) : ¬ is_atom (11^n) :=
+begin
+  unfold is_atom ite, cases le.dest H, 
+  rw nat.add_comm at h, rw [h.symm, factors_of_exp_prime prime_eleven],
+  simp, induction nat.decidable_eq _ _,
+    simp, apply absurd h_1, exact dec_trivial 
+end
 
 def min_fac_pow_of_five_seven {i j : ℕ} : min_fac (5^(i+1) * 7^(j+1)) = 5 := 
 prime_exp_mul_min_fac_is_least_prime dec_trivial prime_five prime_seven (le_add_left _ _) _ (le_add_left _ _)
@@ -124,6 +147,16 @@ have h₂ : min_fac (5^(i+1) * 7^(j+1)) = 5 := prime_exp_mul_min_fac_is_least_pr
         apply is_impl_pow_of_five_seven
   end
 
+def not_impl_pow_eleven (n > 0) : ¬ is_impl (11^n) :=
+begin
+  unfold is_impl ite, cases le.dest H, 
+  rw nat.add_comm at h, rw [h.symm, factors_of_exp_prime prime_eleven],
+  simp, induction nat.decidable_eq _ _,
+    induction or.decidable,
+      simp, cases h_2, repeat {apply absurd h_2, exact dec_trivial},
+    apply absurd h_1, exact dec_trivial
+end
+
 lemma is_impl_has_pow_of_five_seven : ∀ (n : ℕ), n ≠ 0 → is_impl n → ∃ (i j : ℕ), n = 5^i * 7^j
 | 0      := by intro; contradiction 
 | 1      := by intros; fapply exists.intro 0; fapply exists.intro 0; repeat {rw nat.pow_zero}; simp
@@ -158,8 +191,33 @@ lemma is_impl_has_pow_of_five_seven : ∀ (n : ℕ), n ≠ 0 → is_impl n → �
                 rw [nat.pow_succ, (nat.mul_assoc (5^i) _ (7^j)), nat.mul_comm 5 (7^j)],
                 rw [eq.symm (nat.mul_assoc (5^i) (7^j) _), eq.symm h_3],
                 apply eq.symm, apply nat.div_mul_cancel,
-                  rw eq.symm h_1,
+                  rw h_1.symm,
                   apply min_fac_dvd
+  end
+
+def is_box_pow_eleven : ∀ (n : ℕ), is_box (11^n)
+| 0 := by unfold is_box ite
+| (k+1) := by unfold is_box ite; rw factors_of_exp_prime prime_eleven; apply is_box_pow_eleven
+
+lemma is_box_has_pow_of_eleven : ∀ (n : ℕ), n ≠ 0 → is_box n → ∃ (i : ℕ), n = 11^i
+| 0      := by intro; contradiction 
+| 1      := by intros; fapply exists.intro 0; rw nat.pow_zero; simp
+| (k+2)  :=
+  have h₁ : (k+2) / min_fac (k+2) < k+2 := factors_lemma,
+  have h₂ : (k+2) > 0 := lt_trans (zero_lt_succ 0) (le_add_left _ _),
+  begin
+    intro h, unfold is_box ite, rw factors_min_fac (le_add_left _ _),
+    simp, induction nat.decidable_eq _ _,
+      simp, simp, intro h₃,
+      have hn : ∃ (i : ℕ), (k + 2) / min_fac (k + 2) = 11 ^ i := 
+        is_box_has_pow_of_eleven ((k+2) / min_fac (k+2)) (pos_div_min_fac (k+2) h₂) h₃,
+      cases hn with i h_3,
+        rw h_1 at h_3, 
+        fapply exists.intro (i+1),
+          rw nat.pow_succ, rw h_3.symm, 
+          apply eq.symm, apply nat.div_mul_cancel,
+            rw h_1.symm,
+              apply min_fac_dvd
   end
 
 -- our decoding function is well-founded
@@ -206,6 +264,10 @@ begin
       apply pow_ge_one, exact dec_trivial
 end
 
+lemma box_eleven_count_lt (n ≠ 0) : is_box n → count 11 (factors n) < n :=
+by intro h; cases is_box_has_pow_of_eleven n H h with i h₁; 
+  rw [h₁, count_exp_factors prime_eleven]; apply exp_lt_pow; exact dec_trivial
+
 /- decoding of propositional formulas -/
 
 @[reducible]
@@ -221,14 +283,19 @@ def decode_form (σ : nat) : nat → option (form σ)
       option.some (#⟨count 3 (factors n) - 1,h⟩) 
     else
       none
-  else if h : is_impl n 
+  else if h₁ : is_impl n 
     then
-      have count 5 (factors n) < n := impl_five_count_lt _ (succ_ne_zero _) h,
-      have count 7 (factors n) < n := impl_seven_count_lt _ (succ_ne_zero _) h,
+      have count 5 (factors n) < n := impl_five_count_lt _ (succ_ne_zero _) h₁,
+      have count 7 (factors n) < n := impl_seven_count_lt _ (succ_ne_zero _) h₁,
       option.rec_on (decode_form (count 5 (factors n))) none
       (λ p, option.rec_on (decode_form (count 7 (factors n))) none 
         (λ q, some (p ⊃ q)) )
-    else none 
+  else if h₂ : is_box n
+    then
+      have count 11 (factors n) < n := box_eleven_count_lt _ (succ_ne_zero _) h₂,
+      option.rec_on (decode_form (count 11 (factors n))) none
+      (λ p, some (◻p))
+  else none
 
 def decode_form_lemma {n : ℕ} (h : n ≥ 3) :
   decode_form σ n =
@@ -246,7 +313,12 @@ def decode_form_lemma {n : ℕ} (h : n ≥ 3) :
         option.rec_on (decode_form σ (count 5 (factors n))) none
         (λ p, option.rec_on (decode_form σ (count 7 (factors n))) none 
           (λ q, some (p ⊃ q)) )
-      else none 
+    else if h₃ : is_box n
+    then
+      have count 11 (factors n) < n := box_eleven_count_lt _ (by intro hn; cases hn; apply absurd h (not_lt_zero 2)) h₃,
+      option.rec_on (decode_form σ (count 11 (factors n))) none
+      (λ p, some (◻p))
+  else none
  :=
 by cases le.dest h; unfold dite; rw h_1.symm; rw nat.add_comm 3 w at *; unfold decode_form ite dite
 
@@ -272,9 +344,8 @@ match v with
                     induction nat.decidable_lt _ _,
                       simp, rw nat.add_zero 3 at *,
                       rw factors_of_prime prime_three at *,
-                        simp at *, cases eq_or_lt_of_le h_2,
-                          rw h_3 at *, apply absurd h, apply lt_irrefl,
-                          apply nat.lt_asymm h, assumption,
+                        simp at *, rw h_2 at *, 
+                        apply absurd h, apply lt_irrefl,
                       simp, apply fin.eq_of_veq, unfold fin.val,
                         rw factors_of_prime prime_three, simp,
 
@@ -291,6 +362,8 @@ match v with
               end 
 end
 
+-- implication
+
 lemma impl_encode_ge_three {p q : form σ} : 5^(encode_form p) * 7^(encode_form q) ≥ 3 :=
 have h₁ : 3 ≤ 5 := dec_trivial,
 have h₂ : 1 ≤ 5 := dec_trivial,
@@ -303,8 +376,6 @@ begin
           apply le_trans (nat.zero_le 5), apply (pow_le_no_pow h₂ (encode_ge_one p))
 end
 
--- implication
-
 def encodek_impl {p q : form σ} :
   decode_form σ (encode_form p) = some p → 
   decode_form σ (encode_form q) = some q →
@@ -316,7 +387,7 @@ begin
     simp, induction is_impl_dec,
       cases le.dest (encode_ge_one p), rw nat.add_comm at h_2,
         cases le.dest (encode_ge_one q), rw nat.add_comm at h_3,
-          unfold dite, simp, 
+          unfold dite, apply false.rec,        
         apply h_1, induction h_2, induction h_3,
           apply is_impl_pow_of_five_seven,
       unfold dite,
@@ -330,12 +401,34 @@ begin
           apply not_atom_pow_five_seven
 end
 
+-- box
+
+lemma box_encode_ge_three {p : form σ} : 11^(encode_form p) ≥ 3 :=
+have h₁ : 3 ≤ 11 := dec_trivial,
+le_trans h₁ (pow_le_no_pow dec_trivial (encode_ge_one p))
+
+def encodek_box {p : form σ} :
+  decode_form σ (encode_form p) = some p → 
+  decode_form σ (encode_form (◻p)) = some (◻p) :=
+begin
+  intro hp, unfold encode_form,
+  rw decode_form_lemma box_encode_ge_three, unfold ite, 
+  induction is_atom_dec,
+    simp, induction is_impl_dec,
+      unfold dite, induction is_box_dec,
+        apply false.rec, apply h_2,  apply is_box_pow_eleven,
+        simp, rw [count_exp_factors prime_eleven, hp],
+      apply absurd h_1, apply not_impl_pow_eleven _ (encode_ge_one p),
+    apply absurd h, apply not_atom_pow_eleven _ (encode_ge_one p),
+end
+
 -- putting all the pieces together
 
 def encodek_form : ∀ (p : form σ), decode_form σ (encode_form p) = some p
 | (atom v)   := encodek_atom v
 |  (bot σ)   := encodek_bot
 | (impl p q) := encodek_impl (encodek_form p) (encodek_form q)
+| (box p) := encodek_box (encodek_form p)
 
 /- enumeration of all propositional atoms -/
 
