src/encodable2.lean
@@ -1,0 +1,106 @@
+/-
+Copyright (c) 2018 Jeremy Avigad. All rights reserved.
+Released under Apache 2.0 license as described in the file LICENSE.
+Authors: Jeremy Avigad
+-/
+
+import data.equiv.encodable data.equiv.list data.fin data.finset data.fintype
+
+/-
+`Wfin α ar` is the type of finitely branching trees with labels from α, where 
+a node labeled `a` has `ar a` children. 
+-/
+
+inductive Wfin {α : Type*} (ar : α → ℕ)
+| mk (a : α) (f : fin (ar a) → Wfin) : Wfin
+
+namespace Wfin
+
+variables {α : Type*} {ar : α → ℕ}
+
+def depth : Wfin ar → ℕ 
+| ⟨a, f⟩ := finset.sup finset.univ (λ n, depth (f n)) + 1
+
+def not_depth_le_zero (t : Wfin ar) : ¬ t.depth ≤ 0 :=
+by { cases t, apply nat.not_succ_le_zero }
+
+lemma depth_lt_depth_mk (a : α) (f : fin (ar a) → Wfin ar) (i : fin (ar a)) :
+  depth (f i) < depth ⟨a, f⟩ :=
+nat.lt_succ_of_le (finset.le_sup (finset.mem_univ i))
+
+end Wfin
+
+/-
+Show  `Wfin` types are encodable.
+-/
+
+namespace encodable
+
+@[reducible] private def Wfin' {α : Type*} (ar : α → ℕ) (n : ℕ) := 
+{ t : Wfin ar // t.depth ≤ n}
+
+variables {α : Type*} {ar : α → ℕ}
+
+private def encodable_zero : encodable (Wfin' ar 0) :=
+let f    : Wfin' ar 0 → empty := λ ⟨x, h⟩, absurd h (Wfin.not_depth_le_zero _),
+    finv : empty → Wfin' ar 0 := by { intro x, cases x} in
+have ∀ x, finv (f x) = x, from λ ⟨x, h⟩, absurd h (Wfin.not_depth_le_zero _), 
+encodable.of_left_inverse f finv this
+
+private def f (n : ℕ) : Wfin' ar (n + 1) → Σ a : α, fin (ar a) → Wfin' ar n
+| ⟨t, h⟩ := 
+  begin
+    cases t with a f, 
+    have h₀ : ∀ i : fin (ar a), Wfin.depth (f i) ≤ n,
+      from λ i, nat.le_of_lt_succ (lt_of_lt_of_le (Wfin.depth_lt_depth_mk a f i) h),
+    exact ⟨a, λ i : fin (ar a), ⟨f i, h₀ i⟩⟩ 
+  end
+
+private def finv (n : ℕ) : 
+  (Σ a : α, fin (ar a) → Wfin' ar n) → Wfin' ar (n + 1)
+| ⟨a, f⟩ := 
+  let f' := λ i : fin (ar a), (f i).val in
+  have Wfin.depth ⟨a, f'⟩ ≤ n + 1, 
+    from add_le_add_right (finset.sup_le (λ b h, (f b).2)) 1,
+  ⟨⟨a, f'⟩, this⟩  
+
+variable [encodable α]
+
+private def encodable_succ (n : nat) (h : encodable (Wfin' ar n)) :
+  encodable (Wfin' ar (n + 1)) :=
+encodable.of_left_inverse (f n) (finv n)
+  (by { intro t, cases t with t h, cases t with a fn, reflexivity })
+
+instance : encodable (Wfin ar) :=
+begin 
+  haveI h' : Π n, encodable (Wfin' ar n) := 
+    λ n, nat.rec_on n encodable_zero encodable_succ, 
+  let f    : Wfin ar → Σ n, Wfin' ar n   := λ t, ⟨t.depth, ⟨t, le_refl _⟩⟩,
+  let finv : (Σ n, Wfin' ar n) → Wfin ar := λ p, p.2.1,
+  have : ∀ t, finv (f t) = t, from λ t, rfl,
+  exact encodable.of_left_inverse f finv this
+end
+
+end encodable
+
+/-
+Make it easier to construct funtions from a small `fin`.
+-/
+
+namespace fin
+variable {α : Type*}
+
+def mk_fn0 : fin 0 → α 
+| ⟨_, h⟩ := absurd h dec_trivial
+
+def mk_fn1 (t : α) : fin 1 → α
+| ⟨0, _⟩   := t
+| ⟨n+1, h⟩ := absurd h dec_trivial
+
+def mk_fn2 (s t : α) : fin 2 → α
+| ⟨0, _⟩   := s
+| ⟨1, _⟩   := t
+| ⟨n+2, h⟩ := absurd h dec_trivial
+
+attribute [simp] mk_fn0 mk_fn1 mk_fn2
+end fin
