src/mpl/context.lean
@@ -4,7 +4,16 @@ Released under the Apache License 2.0 (see "License");
 Author: Bruno Bentzen
 -/
 
-import .basic ..language.basic
+import .language
+
+/- context -/ 
+
+@[reducible]
+def ctx (σ : nat) : Type := set (form σ)
+
+notation `·` := {}
+notation Γ `⸴` p := set.insert p Γ
+notation Γ `⊔` Δ := set.union Γ Δ
 
 variable {σ : nat}
 
