src/mpl/encoding2.lean
@@ -1,0 +1,49 @@
+/-
+Copyright (c) 2018 Jeremy Avigad. All rights reserved.
+Released under Apache 2.0 license as described in the file LICENSE.
+Authors: Jeremy Avigad
+-/
+
+import ..encodable2 .language 
+
+-- A more concise encoding of form -- Thanks Jeremy!
+
+namespace form
+
+private def constructors (σ : nat) := (var σ) ⊕ unit ⊕ unit ⊕ unit
+
+local notation `catom` v := sum.inl v
+local notation `cbot`    := sum.inr (sum.inl unit.star)
+local notation `cimpl`   := sum.inr (sum.inr (sum.inr unit.star))
+local notation `cbox`    := sum.inr (sum.inr (sum.inl unit.star))
+
+@[simp]
+private def arity (σ : nat) : constructors σ → nat
+| (catom v) := 0
+| cbot      := 0
+| cimpl     := 2
+| cbox      := 1
+
+variable {σ : nat}
+
+private def f : form σ → Wfin (arity σ) 
+| (atom v)   := ⟨catom v, fin.mk_fn0⟩
+| (bot _)    := ⟨cbot, fin.mk_fn0⟩
+| (impl p q) := ⟨cimpl, fin.mk_fn2 (f p) (f q)⟩       
+| (box  p)   := ⟨cbox, fin.mk_fn1 (f p)⟩
+
+private def finv : Wfin (arity σ) → form σ
+| ⟨catom a, fn⟩ := atom a 
+| ⟨cbot, fn⟩    := bot _
+| ⟨cimpl, fn⟩   := impl (finv (fn ⟨0, dec_trivial⟩)) (finv (fn ⟨1, dec_trivial⟩))       
+| ⟨cbox, fn⟩    := box  (finv (fn ⟨0, dec_trivial⟩))        
+
+instance [encodable (var σ)] : encodable (form σ) :=
+begin
+  haveI : encodable (constructors σ) :=
+    by { unfold constructors, apply_instance },
+  exact encodable.of_left_inverse f finv 
+    (by { intro p, induction p; simp [f, finv, *] })
+end
+
+end form
