src/mpl/s4/default.lean
@@ -4,5 +4,5 @@ Released under the Apache License 2.0 (see "License");
 Author: Bruno Bentzen
 -/
 
-import ..nat ..prime .language .context
+import ..default 
 
