src/mpl/s4/semantics/lemmas.lean
@@ -4,47 +4,47 @@ Released under the Apache License 2.0 (see "License");
 Author: Bruno Bentzen
 -/
 
-import .basic
+import .basic ..syntax.lemmas ..misc 
 
 open form classical
 
 variable {σ : nat}
 
-def not_ff_iff_tt {M : 𝓦 ⸴ 𝓡 ⸴ 𝓿} {w : wrld σ} {p : form σ} : (M⦃p⦄w) ≠ ff ↔ (M⦃p⦄w) = tt := by simp
-def not_tt_iff_ff {M : 𝓦 ⸴ 𝓡 ⸴ 𝓿} {w : wrld σ} {p : form σ} : (M⦃p⦄w) ≠ tt ↔ (M⦃p⦄w) = ff := by simp
+def not_ff_iff_tt {M : 𝓦 ⸴ 𝓡 ⸴ 𝓿} {w : wrld σ} {p : form σ} : ((M⦃p⦄w) ≠ ff) ⇔ (M⦃p⦄w) = tt := by simp
+def not_tt_iff_ff {M : 𝓦 ⸴ 𝓡 ⸴ 𝓿} {w : wrld σ} {p : form σ} : (M⦃p⦄w) ≠ tt ⇔ (M⦃p⦄w) = ff := by simp
 
 /- general facts about non-modal logical constants -/
 
 def neg_tt_iff_ff {M : 𝓦 ⸴ 𝓡 ⸴ 𝓿} {w : wrld σ} {p : form σ} :
-  (M⦃~p⦄w) = tt ↔ (M⦃p⦄w) = ff :=
+  (M⦃~p⦄w) = tt ⇔ (M⦃p⦄w) = ff :=
 by unfold form_tt_in_wrld; induction (form_tt_in_wrld M p w); simp; simp
 
 def neg_ff_iff_tt {M : 𝓦 ⸴ 𝓡 ⸴ 𝓿} {w : wrld σ} {p : form σ} :
-  (M⦃~p⦄w) = ff ↔ (M⦃p⦄w) = tt :=
+  (M⦃~p⦄w) = ff ⇔ (M⦃p⦄w) = tt :=
 by unfold form_tt_in_wrld; induction (form_tt_in_wrld M p w); simp; simp
 
 def impl_tt_iff_tt_implies_tt {M : 𝓦 ⸴ 𝓡 ⸴ 𝓿} {w : wrld σ} {p q : form σ} :
-  (M⦃p ⊃ q⦄w) = tt ↔ ((M⦃p⦄w) = tt → (M⦃q⦄w) = tt) :=
+  (M⦃p ⊃ q⦄w) = tt ⇔ ((M⦃p⦄w) = tt ⇒ (M⦃q⦄w) = tt) :=
 by unfold form_tt_in_wrld; induction (form_tt_in_wrld M p w); repeat {induction (form_tt_in_wrld M q w), simp, simp}
 
 def impl_tt_iff_ff_or_tt {M : 𝓦 ⸴ 𝓡 ⸴ 𝓿} {w : wrld σ} {p q : form σ} :
-  (M⦃p ⊃ q⦄w) = tt ↔ ((M⦃p⦄w) = ff ∨ (M⦃q⦄w) = tt) :=
+  (M⦃p ⊃ q⦄w) = tt ⇔ ((M⦃p⦄w) = ff ∨ (M⦃q⦄w) = tt) :=
 by unfold form_tt_in_wrld; induction (form_tt_in_wrld M p w); repeat {induction (form_tt_in_wrld M q w), simp, simp}
 
 def impl_ff_iff_tt_and_tt {M : 𝓦 ⸴ 𝓡 ⸴ 𝓿} {w : wrld σ} {p q : form σ} :
-  (M⦃p ⊃ q⦄w) = ff ↔ ((M⦃p⦄w) = tt ∧ (M⦃q⦄w) = ff) :=
+  (M⦃p ⊃ q⦄w) = ff ⇔ ((M⦃p⦄w) = tt ∧ (M⦃q⦄w) = ff) :=
 by unfold form_tt_in_wrld; induction (form_tt_in_wrld M p w); repeat {induction (form_tt_in_wrld M q w), simp, simp}
 
 def ff_or_tt_and_tt_implies_tt_right {M : 𝓦 ⸴ 𝓡 ⸴ 𝓿} {w : wrld σ} {p q : form σ} :
-  ((M⦃p⦄w) = ff ∨ (M⦃q⦄w) = tt) → (M⦃p⦄w) = tt → (M⦃q⦄w) = tt :=
-by induction (form_tt_in_wrld M p w); repeat {induction (form_tt_in_wrld M q w), simp, simp}
+  ((M⦃p⦄w) = ff ∨ (M⦃q⦄w) = tt) ⇒ (M⦃p⦄w) = tt ⇒ (M⦃q⦄w) = tt :=
+by unfold form_tt_in_wrld; induction (form_tt_in_wrld M p w); repeat {induction (form_tt_in_wrld M q w), simp, simp}
 
 def ff_or_tt_and_tt_implies_tt_left {M : 𝓦 ⸴ 𝓡 ⸴ 𝓿} {w : wrld σ} {p q : form σ} :
-  ((M⦃p⦄w) = tt ∨ (M⦃q⦄w) = ff) → (M⦃q⦄w) = tt → (M⦃p⦄w) = tt :=
-by induction (form_tt_in_wrld M p w); repeat {induction (form_tt_in_wrld M q w), simp, simp}
+  ((M⦃p⦄w) = tt ∨ (M⦃q⦄w) = ff) ⇒ (M⦃q⦄w) = tt ⇒ (M⦃p⦄w) = tt :=
+by unfold form_tt_in_wrld; induction (form_tt_in_wrld M p w); repeat {induction (form_tt_in_wrld M q w), simp, simp}
 
 def or_neq_to_or_eq {M : 𝓦 ⸴ 𝓡 ⸴ 𝓿} {w : wrld σ} {p q : form σ} :
-  ((M⦃p⦄w) ≠ tt ∨ (M⦃q⦄w) ≠ ff) → ((M⦃p⦄w) = ff ∨ (M⦃q⦄w) = tt) :=
+  ((M⦃p⦄w) ≠ tt ∨ (M⦃q⦄w) ≠ ff) ⇒ ((M⦃p⦄w) = ff ∨ (M⦃q⦄w) = tt) :=
 by induction (form_tt_in_wrld M p w); repeat {induction (form_tt_in_wrld M q w), simp, simp}
 
 def bot_is_insatisf {w : wrld σ} : 
@@ -54,7 +54,7 @@ by intro h; cases h; exact (bool.no_confusion h_h)
 /- Modal logical constants (=>) -/
 
 def forall_wrld_tt_nec_tt {M : 𝓦 ⸴ 𝓡 ⸴ 𝓿} {w : wrld σ} {p : form σ} : 
-  (∀ v, w ∈ (𝓦 ▹ M) → v ∈ (𝓦 ▹ M) → (𝓡 ▹ M) w v = tt → (M⦃p⦄v) = tt) → (M⦃◻p⦄w) = tt := 
+  (∀ v, w ∈ (𝓦 ▹ M) → v ∈ (𝓦 ▹ M) → (𝓡 ▹ M) w v = tt → (M⦃p⦄v) = tt) ⇒ (M⦃◻p⦄w) = tt := 
 begin
   intro h, 
   unfold form_tt_in_wrld,
@@ -64,7 +64,7 @@ begin
 end
 
 def exists_wlrd_tt_pos_tt {M : 𝓦 ⸴ 𝓡 ⸴ 𝓿} {w : wrld σ} {p : form σ} : 
-  (∃ v, w ∈ (𝓦 ▹ M) ∧ v ∈ (𝓦 ▹ M) ∧ (𝓡 ▹ M) w v = tt ∧ (M⦃p⦄v) = tt) → (M⦃◇p⦄w) = tt := 
+  (∃ v, w ∈ (𝓦 ▹ M) ∧ v ∈ (𝓦 ▹ M) ∧ (𝓡 ▹ M) w v = tt ∧ (M⦃p⦄v) = tt) ⇒ (M⦃◇p⦄w) = tt := 
 begin
   intro h,
   unfold form_tt_in_wrld,
@@ -84,15 +84,15 @@ end
 /- Modal logical constants (<=) -/
 
 def nec_tt_forall_wrld_tt {M : 𝓦 ⸴ 𝓡 ⸴ 𝓿} {w : wrld σ} {p : form σ} : 
-  (M⦃◻p⦄w) = tt → (∀ v, w ∈ (𝓦 ▹ M) → v ∈ (𝓦 ▹ M) → (𝓡 ▹ M) w v = tt → (M⦃p⦄v) = tt) := 
+  (M⦃◻p⦄w) = tt ⇒ (∀ v, w ∈ (𝓦 ▹ M) → v ∈ (𝓦 ▹ M) → (𝓡 ▹ M) w v = tt → (M⦃p⦄v) = tt) := 
 begin
   unfold form_tt_in_wrld,
   induction (prop_decidable _),
-    simp, simp
+    repeat {simp}
 end
 
 def pos_tt_exists_wlrd_tt {M : 𝓦 ⸴ 𝓡 ⸴ 𝓿} {w : wrld σ} {p : form σ} : 
-  (M⦃◇p⦄w) = tt → (∃ v, w ∈ (𝓦 ▹ M) ∧ v ∈ (𝓦 ▹ M) ∧ (𝓡 ▹ M) w v = tt ∧ (M⦃p⦄v) = tt) := 
+  (M⦃◇p⦄w) = tt ⇒ (∃ v, w ∈ (𝓦 ▹ M) ∧ v ∈ (𝓦 ▹ M) ∧ (𝓡 ▹ M) w v = tt ∧ (M⦃p⦄v) = tt) := 
 begin
   unfold form_tt_in_wrld,
     simp, intro h, apply classical.by_contradiction, intro h',
@@ -112,13 +112,13 @@ begin
 end
 
 def pos_ff_forall_wrld_ff {M : 𝓦 ⸴ 𝓡 ⸴ 𝓿} {w : wrld σ} {p : form σ} : 
-  (M⦃◇p⦄w) = ff → (∀ v, w ∈ (𝓦 ▹ M) → v ∈ (𝓦 ▹ M) → (𝓡 ▹ M) w v = tt → (M⦃p⦄v) = ff) := 
+  (M⦃◇p⦄w) = ff ⇒ (∀ v, w ∈ (𝓦 ▹ M) → v ∈ (𝓦 ▹ M) → (𝓡 ▹ M) w v = tt → (M⦃p⦄v) = ff) := 
 by unfold form_tt_in_wrld; simp; exact id
 
 /- Some facts about K -/
 
 def nec_impl_to_nec_impl_nec {M : 𝓦 ⸴ 𝓡 ⸴ 𝓿} {w : wrld σ} {p q : form σ} : 
-  (M⦃◻(p ⊃ q)⦄w) = tt → (M⦃◻p⦄w) = tt → (M⦃◻q⦄w) = tt := 
+  (M⦃◻(p ⊃ q)⦄w) = tt ⇒ (M⦃◻p⦄w) = tt ⇒ (M⦃◻q⦄w) = tt := 
 begin
   unfold form_tt_in_wrld, simp at *, intros hlpq hlp v wmem vmem rwv,
   apply ff_or_tt_and_tt_implies_tt_right, 
@@ -126,42 +126,47 @@ begin
     apply hlp, repeat {assumption}, 
 end
 
-/-
-def nec_impl_ff_exist_wlrd_ff {M : 𝓦 ⸴ 𝓡 ⸴ 𝓿} {w : wrld σ} {p q : form σ} : 
-  (M⦃◻(p ⊃ q)⦄ w)= ff → (∃ v, w ∈ (𝓦 ▹ M) ∧ v ∈ (𝓦 ▹ M) ∧ (𝓡 ▹ M) w v = tt ∧ (M⦃p⦄v) = tt ∧ (M⦃q⦄v) = ff) := 
-begin
-  unfold form_tt_in_wrld,
-  simp, intro h,
-    apply classical.by_contradiction, intro hn,
-      have nh : ∀ v, ¬ (w ∈ M.wrlds ∧ v ∈ M.wrlds ∧ M.access w v = tt ∧ _ = tt ∧ _ = ff) :=
-        begin
-          apply forall_not_of_not_exists, exact hn
-        end,
-      apply h,
-        intros v wmem vmem rwv, apply or_neq_to_or_eq, 
-          cases ((@decidable.not_and_iff_or_not _ _ (prop_decidable _) (prop_decidable _)).1 (nh v)),
-            contradiction,
-              cases ((@decidable.not_and_iff_or_not _ _ (prop_decidable _) (prop_decidable _)).1 h_1),
-                contradiction,
-                cases ((@decidable.not_and_iff_or_not _ _ (prop_decidable _) (prop_decidable _)).1 h_2),
-                  contradiction,
-                  apply (@decidable.not_and_iff_or_not _ _ (prop_decidable _) (prop_decidable _)).1,
-                    assumption
-end
---/
-
 def nec_nec_to_nec_impl {M : 𝓦 ⸴ 𝓡 ⸴ 𝓿} {w : wrld σ} {p q : form σ} : 
-  (M⦃◻p⦄w) = tt → (M⦃◻q⦄w) = tt → (M⦃◻(p ⊃ q)⦄w) = tt  := 
+  (M⦃◻p⦄w) = tt ⇒ (M⦃◻q⦄w) = tt ⇒ (M⦃◻(p ⊃ q)⦄w) = tt  := 
 begin
   unfold form_tt_in_wrld, simp at *,
   intros hp hq v wmem vmem rwv,
     rw or.comm, apply or.intro_right, apply hq, repeat {assumption}
 end
 
+/- Some facts about T -/
+
+def nec_to_tt {M : 𝓦 ⸴ 𝓡 ⸴ 𝓿} {w : wrld σ} {wm : w ∈ 𝓦 ▹ M} {p : form σ} : -- 
+  (M⦃◻p⦄w) = tt ⇒ (M⦃p⦄w) = tt := 
+begin
+  unfold form_tt_in_wrld, simp at *,
+  intro f, apply f, repeat {assumption}, apply M.refl, assumption
+end
+
+def nec_impl_tt {M : 𝓦 ⸴ 𝓡 ⸴ 𝓿} {w : wrld σ} {w ∈ 𝓦 ▹ M} {p : form σ} : 
+  (M⦃(◻p) ⊃ p⦄w) = tt := 
+by apply impl_tt_iff_tt_implies_tt.2; apply nec_to_tt; repeat {assumption}
+
+/- Some facts about S4 -/
+
+def nec_to_nec_of_nec {M : 𝓦 ⸴ 𝓡 ⸴ 𝓿} {w : wrld σ} {p : form σ} : 
+  (M⦃◻p⦄w) = tt ⇒ (M⦃◻◻p⦄w) = tt := 
+begin
+  unfold form_tt_in_wrld, simp at *,
+  intros f v wmem vmem rwv u vmem' umem rvu,
+    apply f, repeat {assumption},
+      apply M.trans, assumption, exact vmem, 
+        repeat {assumption}
+end
+
+def nec_impl_nec_of_nec {M : 𝓦 ⸴ 𝓡 ⸴ 𝓿} {w : wrld σ} {p : form σ} : 
+  (M⦃(◻p) ⊃ ◻◻p⦄w) = tt := 
+by apply impl_tt_iff_tt_implies_tt.2; apply nec_to_nec_of_nec; repeat {assumption}
+
 /- general facts about contexts -/ 
 
 def ctx_tt_iff_mem_tt {Γ : ctx σ} {M : 𝓦 ⸴ 𝓡 ⸴ 𝓿} {w : wrld σ} :
-  (M⦃Γ⦄w) = tt ↔ (∀ p, p ∈ Γ → (M⦃p⦄w) = tt) :=
+  (M⦃Γ⦄w) = tt ⇔ (∀ p, p ∈ Γ ⇒ (M⦃p⦄w) = tt) :=
 begin
   unfold ctx_tt_in_wrld,
   induction (classical.prop_decidable _),
@@ -172,17 +177,17 @@ begin
 end
 
 def mem_tt_to_ctx_tt (Γ : ctx σ) {M : 𝓦 ⸴ 𝓡 ⸴ 𝓿} {w : wrld σ} :
- (∀ (p : form σ) (h : p ∈ Γ), (M⦃p⦄w) = tt) → (M⦃Γ⦄w) = tt :=
+ (∀ (p : form σ) (h : p ∈ Γ), (M⦃p⦄w) = tt) ⇒ (M⦃Γ⦄w) = tt :=
 ctx_tt_iff_mem_tt.2
 
 def ctx_tt_to_mem_tt {Γ : ctx σ} {M : 𝓦 ⸴ 𝓡 ⸴ 𝓿} {w : wrld σ} {p : form σ} :
-  (M⦃Γ⦄w) = tt → p ∈ Γ → (M⦃p⦄w) = tt :=
+  (M⦃Γ⦄w) = tt ⇒ p ∈ Γ ⇒ (M⦃p⦄w) = tt :=
 by intro; apply ctx_tt_iff_mem_tt.1; assumption
 
 /- context projections -/
 
 def cons_ctx_tt_iff_and {Γ : ctx σ} {M : 𝓦 ⸴ 𝓡 ⸴ 𝓿} {w : wrld σ} {p : form σ} : 
-  (M⦃(Γ ⸴ p)⦄w) = tt ↔ (M⦃Γ⦄w) = tt ∧ (M⦃p⦄w) = tt :=
+  (M⦃(Γ ⸴ p)⦄w) = tt ⇔ (M⦃Γ⦄w) = tt ∧ (M⦃p⦄w) = tt :=
 begin
   unfold ctx_tt_in_wrld,
   induction (classical.prop_decidable (∀ p, p ∈ Γ → form_tt_in_wrld M p w = tt)),
@@ -207,17 +212,17 @@ begin
 end
 
 def cons_ctx_tt_to_ctx_tt {Γ : ctx σ} {M : 𝓦 ⸴ 𝓡 ⸴ 𝓿} {w : wrld σ} {p : form σ} : 
-  (M⦃(Γ ⸴ p)⦄w) = tt → (M⦃Γ⦄w) = tt :=
+  (M⦃(Γ ⸴ p)⦄w) = tt ⇒ (M⦃Γ⦄w) = tt :=
 by intro h; apply and.elim_left; apply cons_ctx_tt_iff_and.1 h
 
 def ctx_tt_cons_tt_to_cons_ctx_tt {Γ : ctx σ} {M : 𝓦 ⸴ 𝓡 ⸴ 𝓿} {w : wrld σ} {p : form σ} : 
-  (M⦃Γ⦄w) = tt → (M⦃p⦄w) = tt  → (M⦃(Γ ⸴ p)⦄w) = tt :=
+  (M⦃Γ⦄w) = tt ⇒ (M⦃p⦄w) = tt  ⇒ (M⦃(Γ ⸴ p)⦄w) = tt :=
 by intros hg hp; apply cons_ctx_tt_iff_and.2; split; assumption; assumption
 
 /- sub-contexts -/
 
 def ctx_tt_to_subctx_tt {Γ Δ : ctx σ} {M : 𝓦 ⸴ 𝓡 ⸴ 𝓿} {w : wrld σ} : 
-  (M⦃Γ⦄w) = tt → Δ ⊆ Γ → (M⦃Δ⦄w) = tt :=
+  (M⦃Γ⦄w) = tt ⇒ Δ ⊆ Γ ⇒ (M⦃Δ⦄w) = tt :=
 begin
   intros h s, 
     apply ctx_tt_iff_mem_tt.2, 
@@ -229,14 +234,14 @@ end
 /- the deduction metatheorem -/
 
 def sem_deduction {Γ : ctx σ} {p q : form σ} :
-  (Γ ⸴ p ⊨ₖ q) → (Γ ⊨ₖ p ⊃ q) :=
+  (Γ ⸴ p ⊨ₛ₄ q) ⇒ (Γ ⊨ₛ₄ p ⊃ q) :=
 begin
  intro h,
  cases h,
    apply sem_csq.is_true,
-     intros M w ant,
+     intros M w wmem ant,
      apply impl_tt_iff_tt_implies_tt.2,
-       intro hp, apply h,
+       intro hp, apply h, assumption, 
          apply ctx_tt_cons_tt_to_cons_ctx_tt,
            repeat {assumption}
 end
