src/mpl/s4/soundness.lean
@@ -4,14 +4,14 @@ Released under the Apache License 2.0 (see "License");
 Author: Bruno Bentzen
 -/
 
-import .syntax.lemmas .semantics.lemmas 
+import ..default .syntax.lemmas .semantics.lemmas
 
 variable {σ : nat}
 
 /- soundness -/
 
 definition sndnss {Γ : ctx σ} {p : form σ} :
-  (Γ ⊢ₖ p) → (Γ ⊨ₖ p) :=
+  (Γ ⊢ₛ₄ p) ⇒ (Γ ⊨ₛ₄ p) :=
 begin
   intro h,
   induction h,
@@ -21,7 +21,7 @@ begin
           repeat {assumption},
     repeat {
       apply sem_csq.is_true,
-        intros M w ctt,
+        intros M w wmem ctt,
         unfold form_tt_in_wrld,
           induction (form_tt_in_wrld M h_p w),
             repeat {
@@ -31,21 +31,20 @@ begin
     },
           induction (form_tt_in_wrld M h_r w),
                 simp, simp,
-
-    apply sem_csq.is_true, -- mp
+    apply sem_csq.is_true,
       induction h_ih_hpq,
         induction h_ih_hp,
-          intros M w ctt,
+          intros M w wmem ctt,
             revert h_ih_hpq,
             unfold form_tt_in_wrld, simp,
             intro hpq,
-            cases (hpq M w ctt),
-             assumption,
-             apply false.rec,
-               exact (bool.no_confusion (eq.trans (eq.symm (h_ih_hp M w ctt)) h)),
-             
+            cases (hpq M w wmem ctt),
+              assumption,
+              apply false.rec,
+                exact (bool.no_confusion (eq.trans (eq.symm (h_ih_hp M w wmem ctt)) h)),
+
     apply sem_csq.is_true, -- k
-      intros M w ctt,
+      intros M w wmem ctt,
       apply impl_tt_iff_tt_implies_tt.2,
         intro lpq, apply impl_tt_iff_tt_implies_tt.2,
           revert lpq, unfold form_tt_in_wrld, simp,
@@ -53,14 +52,22 @@ begin
             cases (lpq v wmem vmem rwv),
               assumption,
               exact (bool.no_confusion (eq.trans (eq.symm (lp v wmem vmem rwv)) h)),
-              
-    apply sem_csq.is_true, -- nec
+
+    apply sem_csq.is_true, -- t
+      intros M w wmem ctt,
+      apply nec_impl_tt, repeat {assumption},
+    
+    apply sem_csq.is_true, -- s4
+      intros M w wmem ctt,
+      apply nec_impl_nec_of_nec,
+    
+    apply sem_csq.is_true,
       induction h_ih,
-        intros M w ctt,
+        intros M w wmem ctt,
         unfold form_tt_in_wrld, simp,
         intros v wmem vmem rwv,
-          apply h_ih,
-            apply eq.substr h_cnil,
+          apply h_ih, assumption,
+            rw h_cnil, 
               unfold ctx_tt_in_wrld,
-              simp--, intros, apply false.rec, assumption
+              simp, --intros, apply false.rec, assumption
 end
