src/mpl/s4/syntax/basic.lean
@@ -4,11 +4,11 @@ Released under the Apache License 2.0 (see "License");
 Author: Bruno Bentzen
 -/
 
-import ..default 
+import ..default
 
 variable {σ : nat}
 
-/- the K system -/
+/- the S4 system -/
 
 inductive prf (Γ : ctx σ) : form σ → Prop
 | ax {p : form σ} (h : p ∈ Γ) : prf p
@@ -17,13 +17,15 @@ inductive prf (Γ : ctx σ) : form σ → Prop
 | pl3 {p q : form σ} :  prf (((~p) ⊃ ~q) ⊃ (((~p) ⊃ q) ⊃ p))
 | mp {p q : form σ} (hpq: prf (p ⊃ q)) (hp : prf p) : prf q
 | k  {p q : form σ} : prf ((◻(p ⊃ q)) ⊃ ((◻p) ⊃ (◻q)))
+| t  {p : form σ} : prf ((◻p) ⊃ p)
+| s4 {p : form σ} : prf ((◻p) ⊃ ◻◻p)
 | nec {p : form σ} (cnil : Γ = ·) (h : prf p) : prf (◻p)
 
 axiom nec_weak {Γ Δ : ctx σ} {p : form σ} (h : Δ ⊆ Γ) :
   (prf Δ ◻p) → (prf Γ ◻p)
 
-notation Γ `⊢ₖ` p := prf Γ p
-notation Γ `⊬ₖ` p := prf Γ p → false
+notation Γ `⊢ₛ₄` p := prf Γ p
+notation Γ `⊬ₛ₄` p := prf Γ p → false
 
 /- metaconnectives -/
 
