src/pl/semantics/lemmas.lean
@@ -6,61 +6,61 @@ Author: Bruno Bentzen
 
 import .basic
 
+open form
+
 variable {σ : nat}
 
 /- general facts about the logical constants -/
 
 def neg_tt_iff_ff {v : var σ → bool} {p : form σ} :
-  (⦃~p⦄v) = tt ⇔ (⦃p⦄v) = ff :=
+  (⦃~p⦄v) = tt ↔ (⦃p⦄v) = ff :=
 by unfold form_tt_in_val; induction (form_tt_in_val v p); simp; simp
 
 def neg_ff_iff_tt {v : var σ → bool} {p : form σ} :
-  (⦃~p⦄v) = ff ⇔ (⦃p⦄v) = tt :=
+  (⦃~p⦄v) = ff ↔ (⦃p⦄v) = tt :=
 by unfold form_tt_in_val; induction (form_tt_in_val v p); simp; simp
 
 def impl_tt_iff_tt_implies_tt {v : var σ → bool} {p q : form σ} :
-  (⦃p ⊃ q⦄v) = tt ⇔ ((⦃p⦄v) = tt ⇒ (⦃q⦄v) = tt) :=
+  (⦃p ⊃ q⦄v) = tt ↔ ((⦃p⦄v) = tt → (⦃q⦄v) = tt) :=
 by unfold form_tt_in_val; induction (form_tt_in_val v p); repeat { induction (form_tt_in_val v q), simp, simp }
 
 def impl_tt_iff_ff_or_tt {v : var σ → bool} {p q : form σ} :
-  (⦃p ⊃ q⦄v) = tt ⇔ ((⦃p⦄v) = ff ∨ (⦃q⦄v) = tt) :=
+  (⦃p ⊃ q⦄v) = tt ↔ ((⦃p⦄v) = ff ∨ (⦃q⦄v) = tt) :=
 by unfold form_tt_in_val; induction (form_tt_in_val v p); repeat { induction (form_tt_in_val v q), simp, simp }
 
 def impl_ff_iff_tt_and_tt {v : var σ → bool} {p q : form σ} :
-  (⦃p ⊃ q⦄v) = ff ⇔ ((⦃p⦄v) = tt ∧ (⦃q⦄v) = ff) :=
+  (⦃p ⊃ q⦄v) = ff ↔ ((⦃p⦄v) = tt ∧ (⦃q⦄v) = ff) :=
 by unfold form_tt_in_val; induction (form_tt_in_val v p); repeat { induction (form_tt_in_val v q), simp, simp }
 
 def bot_is_insatisf : 
-  ¬ ∃ (v : var σ → bool), (⦃⊥⦄ v) = tt :=
+  ¬ ∃ (v : var σ → bool), (⦃bot σ⦄ v) = tt :=
 by intro h; cases h; exact (bool.no_confusion h_h) 
 
 /- general facts about contexts -/ 
 
 def ctx_tt_iff_mem_tt {Γ : ctx σ} {v : var σ → bool} :
-  (⦃Γ⦄v) = tt ⇔ (∀ p, p ∈ Γ ⇒ (⦃p⦄v) = tt) :=
+  (⦃Γ⦄v) = tt ↔ (∀ p, p ∈ Γ → (⦃p⦄v) = tt) :=
 begin
   unfold ctx_tt_in_val,
   induction (classical.prop_decidable _),
-    repeat {
       apply iff.intro,
-        repeat {
-          simp, intro, assumption
-        } 
-    }
+          simp, intro,
+          simp, assumption,
+          simp
 end
 
 def mem_tt_to_ctx_tt (Γ : ctx σ) {v : var σ → bool} :
- (∀ (p : form σ) (h : p ∈ Γ), (⦃p⦄ v) = tt) ⇒ (⦃Γ⦄ v) = tt :=
+ (∀ (p : form σ) (h : p ∈ Γ), (⦃p⦄ v) = tt) → (⦃Γ⦄ v) = tt :=
 ctx_tt_iff_mem_tt.2
 
 def ctx_tt_to_mem_tt {Γ : ctx σ} {p : form σ} {v : var σ → bool} :
-  (⦃Γ⦄v) = tt ⇒ p ∈ Γ ⇒ (⦃p⦄v) = tt :=
+  (⦃Γ⦄v) = tt → p ∈ Γ → (⦃p⦄v) = tt :=
 by intro; apply ctx_tt_iff_mem_tt.1; assumption
 
 /- context projections -/
 
 def cons_ctx_tt_iff_and {Γ : ctx σ} {p : form σ} {v : var σ → bool} :
-  (⦃(Γ ⸴ p)⦄v) = tt ⇔ (⦃Γ⦄v) = tt ∧ (⦃p⦄v) = tt :=
+  (⦃(Γ ⸴ p)⦄v) = tt ↔ (⦃Γ⦄v) = tt ∧ (⦃p⦄v) = tt :=
 begin
   unfold ctx_tt_in_val,
   induction (classical.prop_decidable (∀ p, p ∈ Γ → form_tt_in_val v p = tt)),
@@ -84,17 +84,17 @@ begin
 end
 
 def cons_ctx_tt_to_ctx_tt {Γ : ctx σ} {p : form σ} {v : var σ → bool} :
-  (⦃(Γ ⸴ p)⦄v) = tt ⇒ (⦃Γ⦄v) = tt :=
+  (⦃(Γ ⸴ p)⦄v) = tt → (⦃Γ⦄v) = tt :=
 by intro h; apply and.elim_left; apply cons_ctx_tt_iff_and.1 h
 
 def ctx_tt_cons_tt_to_cons_ctx_tt {Γ : ctx σ} {p : form σ} {v : var σ → bool} :
-  (⦃Γ⦄v) = tt ⇒ (⦃p⦄v) = tt  ⇒ (⦃(Γ ⸴ p)⦄v) = tt :=
+  (⦃Γ⦄v) = tt → (⦃p⦄v) = tt  → (⦃(Γ ⸴ p)⦄v) = tt :=
 by intros hg hp; apply cons_ctx_tt_iff_and.2; split; assumption; assumption
 
 /- sub-contexts -/
 
 def ctx_tt_to_subctx_tt {Γ Δ : ctx σ} {v : var σ → bool} :
-  (⦃Γ⦄v) = tt ⇒ Δ ⊆ Γ ⇒ (⦃Δ⦄v) = tt :=
+  (⦃Γ⦄v) = tt → Δ ⊆ Γ → (⦃Δ⦄v) = tt :=
 begin
   intros h s, 
     apply ctx_tt_iff_mem_tt.2, 
@@ -106,7 +106,7 @@ end
 /- useful metatheorems -/
 
 def sem_deduction {Γ : ctx σ} {p q : form σ} :
-  (Γ ⸴ p ⊨ₚ q) ⇒ (Γ ⊨ₚ p ⊃ q) :=
+  (Γ ⸴ p ⊨ₚ q) → (Γ ⊨ₚ p ⊃ q) :=
 begin
  intro h,
  cases h,
@@ -121,7 +121,7 @@ begin
 end
 
 def sum_weak {Γ : ctx σ} {p q r : form σ} :
-  (Γ ⊨ₚ p) ⇒ (Γ ⸴ q ⊨ₚ p) :=
+  (Γ ⊨ₚ p) → (Γ ⸴ q ⊨ₚ p) :=
 begin
   intro h,
     cases h,
