src/pl/syntax/basic.lean
@@ -4,7 +4,7 @@ Released under the Apache License 2.0 (see "License");
 Author: Bruno Bentzen
 -/
 
-import .language.basic .context.basic
+import ..context
 
 variable {σ : nat}
 
